Veir/Passes/InstructionSelection/Proofs.lean
@@ -36,6 +36,29 @@ theorem helper2 {i : LLVM.Int w} :
     (LLVM.Int.toReg i).val = i.getValueD.zeroExtend 64 := by
   cases i <;> simp [llvm_toBitVec, reg_toBitVec, LLVM.Int.toReg, LLVM.Int.getValueD]
 
+@[reg_toBitVec, grind =]
+theorem helper5 {i : LLVM.Int w} (h : i.isPoison = false := by grind) :
+    (LLVM.Int.toReg i).val = i.getValue.zeroExtend 64 := by
+  cases i <;>
+  simp [llvm_toBitVec, reg_toBitVec, LLVM.Int.toReg, LLVM.Int.getValue]
+  split
+  simp_all
+
+theorem BitVec.ult_one_iff_of_lt {lhs : BitVec w} (h : 0 < w) :
+    (lhs.ult 1#w) = decide (lhs = 0#w) := by
+  simp only [BitVec.ult_eq_decide, BitVec.toNat_ofNat, decide_eq_decide]
+  rw [Nat.mod_eq_of_lt (by grind)]
+  simp [← BitVec.toNat_inj]
+
+theorem BitVec.ult_zero_false {lhs : BitVec w} :
+    (0#w).ult lhs = decide (¬lhs = 0#w) := by
+  by_cases hzero : lhs = 0#w
+  · simp [hzero, BitVec.ult]
+  · by_cases hlt : (0#w).ult lhs
+    · simp [hlt, hzero]
+    · simp [BitVec.ult_eq_decide] at hlt
+      simp [BitVec.ult_eq_decide, hlt, ← BitVec.toNat_inj]
+
 /--
   Prove the correctness of the `constant` lowering pattern.
 
@@ -49,41 +72,283 @@ theorem constant_refinement:
 /--
   Prove the correctness of the `add` lowering pattern.
 -/
-theorem add_refinement:
-    (Data.LLVM.Int.add x y) ⊒ (RISCV.Reg.toInt (Data.RISCV.add (LLVM.Int.toReg x) (LLVM.Int.toReg y)) 64) := by
-  simp [llvm_toBitVec, reg_toBitVec]
+theorem add_refinement {lhs rhs : LLVM.Int 64} :
+    (Data.LLVM.Int.add lhs rhs) ⊒ (RISCV.Reg.toInt (Data.RISCV.add (LLVM.Int.toReg rhs) (LLVM.Int.toReg lhs)) 64) := by
+  simp only [llvm_toBitVec, reg_toBitVec]
   simp only [LLVM.Int.getValue_eq_getValueD]
-  intros
-
   bv_decide
 
 /--
   Prove the correctness of the `and` lowering pattern.
 -/
-theorem and_refinement:
-    (Data.LLVM.Int.and x y) ⊒ (RISCV.Reg.toInt (Data.RISCV.and (LLVM.Int.toReg x) (LLVM.Int.toReg y)) 64) := by
-  simp [llvm_toBitVec, reg_toBitVec]
+theorem and_refinement{lhs rhs : LLVM.Int 64} :
+    (Data.LLVM.Int.and lhs rhs) ⊒ (RISCV.Reg.toInt (Data.RISCV.and (LLVM.Int.toReg rhs) (LLVM.Int.toReg lhs)) 64) := by
+  simp only [llvm_toBitVec, reg_toBitVec]
   simp only [LLVM.Int.getValue_eq_getValueD]
   bv_decide
 
 /--
   Prove the correctness of the `ashr` lowering pattern.
 -/
-theorem ashr_refinement:
-    (Data.LLVM.Int.ashr x y) ⊒ (RISCV.Reg.toInt (Data.RISCV.sra (LLVM.Int.toReg y) (LLVM.Int.toReg x)) 64) := by
-  simp [llvm_toBitVec, reg_toBitVec]
+theorem ashr_refinement {lhs rhs : LLVM.Int 64} :
+    (Data.LLVM.Int.ashr lhs rhs) ⊒ (RISCV.Reg.toInt (Data.RISCV.sra (LLVM.Int.toReg rhs) (LLVM.Int.toReg lhs)) 64) := by
+  simp only [llvm_toBitVec, reg_toBitVec]
   simp only [LLVM.Int.getValue_eq_getValueD]
-  intros h1 h2
-  rw [Nat.mod_eq_of_lt (by
-      cases y <;> simp [h1, LLVM.Int.getValueD] at *;
-      exact Nat.lt_of_succ_le h2)]
+  simp
+  intros
+  rw [Nat.mod_eq_of_lt (by simp [BitVec.lt_def] at *; grind)]
 
 /--
   Prove the correctness of the `icmp` lowering pattern with `eq`.
 -/
-theorem icmp_refinement:
-    (Data.LLVM.Int.icmp x y LLVM.IntPred.eq) ⊒
-      (RISCV.Reg.toInt (Data.RISCV.sltiu 1#12 (Data.RISCV.xor (LLVM.Int.toReg y) (LLVM.Int.toReg x))) 1) := by
-  simp [llvm_toBitVec, reg_toBitVec]
+theorem icmp_refinement_eq {lhs rhs : LLVM.Int 64} :
+    (Data.LLVM.Int.icmp lhs rhs LLVM.IntPred.eq) ⊒
+      (RISCV.Reg.toInt (Data.RISCV.sltiu 1#12 (Data.RISCV.xor (LLVM.Int.toReg rhs) (LLVM.Int.toReg lhs))) 1) := by
+  simp only [llvm_toBitVec, reg_toBitVec]
+  simp only [LLVM.Int.getValue_eq_getValueD]
+  bv_decide
 
-  sorry
+/--
+  Prove the correctness of the `icmp` lowering pattern with `ne`.
+-/
+theorem icmp_refinement_ne {lhs rhs : LLVM.Int 64} :
+    (Data.LLVM.Int.icmp lhs rhs LLVM.IntPred.ne) ⊒
+      (RISCV.Reg.toInt (Data.RISCV.sltu (Data.RISCV.xor (LLVM.Int.toReg rhs) (LLVM.Int.toReg lhs)) (Data.RISCV.li 0#64)) 1) := by
+  simp only [llvm_toBitVec, reg_toBitVec]
+  simp only [LLVM.Int.getValue_eq_getValueD]
+  simp [BitVec.ult_zero_false]
+  bv_decide
+
+/--
+  Prove the correctness of the `icmp` lowering pattern with `slt`.
+-/
+theorem icmp_refinement_slt {lhs rhs : LLVM.Int 64} :
+    (Data.LLVM.Int.icmp lhs rhs LLVM.IntPred.slt) ⊒
+      (RISCV.Reg.toInt (Data.RISCV.slt (LLVM.Int.toReg rhs) (LLVM.Int.toReg lhs)) 1) := by
+  simp only [llvm_toBitVec, reg_toBitVec]
+  simp only [LLVM.Int.getValue_eq_getValueD]
+  bv_decide
+
+/--
+  Prove the correctness of the `icmp` lowering pattern with `sle`.
+-/
+theorem icmp_refinement_sle {lhs rhs : LLVM.Int 64} :
+    (Data.LLVM.Int.icmp lhs rhs LLVM.IntPred.sle) ⊒
+      (RISCV.Reg.toInt (Data.RISCV.xori 1#12 (Data.RISCV.slt (LLVM.Int.toReg lhs) (LLVM.Int.toReg rhs))) 1) := by
+  simp [llvm_toBitVec, reg_toBitVec]
+  simp only [LLVM.Int.getValue_eq_getValueD]
+  bv_decide
+
+/--
+  Prove the correctness of the `icmp` lowering pattern with `sgt`.
+-/
+theorem icmp_refinement_sgt {lhs rhs : LLVM.Int 64} :
+    (Data.LLVM.Int.icmp lhs rhs LLVM.IntPred.sgt) ⊒
+      (RISCV.Reg.toInt (Data.RISCV.slt (LLVM.Int.toReg lhs) (LLVM.Int.toReg rhs)) 1) := by
+  simp [llvm_toBitVec, reg_toBitVec]
+  simp only [LLVM.Int.getValue_eq_getValueD]
+  bv_decide
+
+/--
+  Prove the correctness of the `icmp` lowering pattern with `sge`.
+-/
+theorem icmp_refinement_sge {lhs rhs : LLVM.Int 64} :
+    (Data.LLVM.Int.icmp lhs rhs LLVM.IntPred.sge) ⊒
+      (RISCV.Reg.toInt (Data.RISCV.xori 1#12 (Data.RISCV.slt (LLVM.Int.toReg rhs) (LLVM.Int.toReg lhs))) 1) := by
+  simp [llvm_toBitVec, reg_toBitVec]
+  simp only [LLVM.Int.getValue_eq_getValueD]
+  bv_decide
+
+/--
+  Prove the correctness of the `icmp` lowering pattern with `ult`.
+-/
+theorem icmp_refinement_ult {lhs rhs : LLVM.Int 64} :
+    (Data.LLVM.Int.icmp lhs rhs LLVM.IntPred.ult) ⊒
+      (RISCV.Reg.toInt (Data.RISCV.sltu (LLVM.Int.toReg rhs) (LLVM.Int.toReg lhs)) 1) := by
+  simp [llvm_toBitVec, reg_toBitVec]
+  simp only [LLVM.Int.getValue_eq_getValueD]
+  bv_decide
+
+/--
+  Prove the correctness of the `icmp` lowering pattern with `ule`.
+-/
+theorem icmp_refinement_ule {lhs rhs : LLVM.Int 64} :
+    (Data.LLVM.Int.icmp lhs rhs LLVM.IntPred.ule) ⊒
+      (RISCV.Reg.toInt (Data.RISCV.xori 1#12 (Data.RISCV.sltu (LLVM.Int.toReg lhs) (LLVM.Int.toReg rhs))) 1) := by
+  simp [llvm_toBitVec, reg_toBitVec]
+  simp only [LLVM.Int.getValue_eq_getValueD]
+  bv_decide
+
+/--
+  Prove the correctness of the `icmp` lowering pattern with `ugt`.
+-/
+theorem icmp_refinement_ugt {lhs rhs : LLVM.Int 64} :
+    (Data.LLVM.Int.icmp lhs rhs LLVM.IntPred.ugt) ⊒
+      (RISCV.Reg.toInt ((Data.RISCV.sltu (LLVM.Int.toReg lhs) (LLVM.Int.toReg rhs))) 1) := by
+  simp [llvm_toBitVec, reg_toBitVec]
+  simp only [LLVM.Int.getValue_eq_getValueD]
+  bv_decide
+
+/--
+  Prove the correctness of the `icmp` lowering pattern with `uge`.
+-/
+theorem icmp_refinement_uge {lhs rhs : LLVM.Int 64} :
+    (Data.LLVM.Int.icmp lhs rhs LLVM.IntPred.uge) ⊒
+      (RISCV.Reg.toInt (Data.RISCV.xori 1#12 (Data.RISCV.sltu (LLVM.Int.toReg rhs) (LLVM.Int.toReg lhs))) 1) := by
+  simp [llvm_toBitVec, reg_toBitVec]
+  simp only [LLVM.Int.getValue_eq_getValueD]
+  bv_decide
+
+/--
+  Prove the correctness of the `or` lowering pattern.
+-/
+theorem or_refinement{lhs rhs : LLVM.Int 64} :
+    (Data.LLVM.Int.or lhs rhs) ⊒ (RISCV.Reg.toInt (Data.RISCV.or (LLVM.Int.toReg rhs) (LLVM.Int.toReg lhs)) 64) := by
+  simp only [llvm_toBitVec, reg_toBitVec]
+  simp only [LLVM.Int.getValue_eq_getValueD]
+  bv_decide
+
+/--
+  Prove the correctness of the `xor` lowering pattern.
+-/
+theorem xor_refinement{lhs rhs : LLVM.Int 64} :
+    (Data.LLVM.Int.xor lhs rhs) ⊒ (RISCV.Reg.toInt (Data.RISCV.xor (LLVM.Int.toReg rhs) (LLVM.Int.toReg lhs)) 64) := by
+  simp only [llvm_toBitVec, reg_toBitVec]
+  simp only [LLVM.Int.getValue_eq_getValueD]
+  bv_decide
+
+/--
+  Prove the correctness of the `mul` lowering pattern.
+-/
+theorem mul_refinement{lhs rhs : LLVM.Int 64} :
+    (Data.LLVM.Int.mul lhs rhs) ⊒ (RISCV.Reg.toInt (Data.RISCV.mul (LLVM.Int.toReg rhs) (LLVM.Int.toReg lhs)) 64) := by
+  simp only [llvm_toBitVec, reg_toBitVec]
+  simp only [LLVM.Int.getValue_eq_getValueD]
+  bv_decide
+
+/--
+  Prove the correctness of the `sdiv` lowering pattern.
+-/
+theorem sdiv_refinement{lhs rhs : LLVM.Int 64} :
+    (Data.LLVM.Int.sdiv lhs rhs) ⊒ (RISCV.Reg.toInt (Data.RISCV.div (LLVM.Int.toReg rhs) (LLVM.Int.toReg lhs)) 64) := by
+  simp only [llvm_toBitVec, reg_toBitVec]
+  simp only [LLVM.Int.getValue_eq_getValueD]
+  simp
+  bv_decide
+
+/--
+  Prove the correctness of the `udiv` lowering pattern.
+-/
+theorem udiv_refinement{lhs rhs : LLVM.Int 64} :
+    (Data.LLVM.Int.udiv lhs rhs) ⊒ (RISCV.Reg.toInt (Data.RISCV.divu (LLVM.Int.toReg rhs) (LLVM.Int.toReg lhs)) 64) := by
+  simp only [llvm_toBitVec, reg_toBitVec]
+  simp only [LLVM.Int.getValue_eq_getValueD]
+  simp
+  bv_decide
+
+/--
+  Prove the correctness of the `udiv` lowering pattern.
+-/
+theorem srem_refinement{lhs rhs : LLVM.Int 64} :
+    (Data.LLVM.Int.srem lhs rhs) ⊒ (RISCV.Reg.toInt (Data.RISCV.rem (LLVM.Int.toReg rhs) (LLVM.Int.toReg lhs)) 64) := by
+  simp only [llvm_toBitVec, reg_toBitVec]
+  simp only [LLVM.Int.getValue_eq_getValueD]
+  bv_decide
+
+/--
+  Prove the correctness of the `udiv` lowering pattern.
+-/
+theorem urem_refinement{lhs rhs : LLVM.Int 64} :
+    (Data.LLVM.Int.urem lhs rhs) ⊒ (RISCV.Reg.toInt (Data.RISCV.remu (LLVM.Int.toReg rhs) (LLVM.Int.toReg lhs)) 64) := by
+  simp only [llvm_toBitVec, reg_toBitVec]
+  simp only [LLVM.Int.getValue_eq_getValueD]
+  bv_decide
+
+/--
+  Prove the correctness of the `udiv` lowering pattern.
+-/
+theorem sub_refinement{lhs rhs : LLVM.Int 64} :
+    (Data.LLVM.Int.sub lhs rhs) ⊒ (RISCV.Reg.toInt (Data.RISCV.sub (LLVM.Int.toReg rhs) (LLVM.Int.toReg lhs)) 64) := by
+  simp only [llvm_toBitVec, reg_toBitVec]
+  simp only [LLVM.Int.getValue_eq_getValueD]
+  bv_decide
+
+/--
+  Prove the correctness of the `sext` lowering pattern, with input width `i8`.
+-/
+theorem sext_refinement_8 {lhs : LLVM.Int 8} (h : 8 < w₂) (h' : w₂ ≤ 64) :
+    (Data.LLVM.Int.sext lhs w₂ h) ⊒ (RISCV.Reg.toInt (Data.RISCV.sextb (LLVM.Int.toReg lhs)) w₂) := by
+  simp only [llvm_toBitVec, reg_toBitVec]
+  simp only [LLVM.Int.getValue_eq_getValueD]
+  simp
+  intro h2
+  simp [LLVM.Int.getValueD]
+  split
+  · simp [LLVM.Int.isPoison] at h2
+  · ext k hk
+    simp [BitVec.getLsbD_signExtend, BitVec.getElem_signExtend]
+    split
+    · simp [show k < 64 by omega, show k ≤ 7 by omega, ← BitVec.getLsbD_eq_getElem]
+    · simp [show k < 64 by omega]
+      bv_decide
+
+/--
+  Prove the correctness of the `sext` lowering pattern, with input width `i16`.
+-/
+theorem sext_refinement_16 {lhs : LLVM.Int 16} (h : 16 < w₂) (h' : w₂ ≤ 64) :
+    (Data.LLVM.Int.sext lhs w₂ h) ⊒ (RISCV.Reg.toInt (Data.RISCV.sexth (LLVM.Int.toReg lhs)) w₂) := by
+  simp only [llvm_toBitVec, reg_toBitVec]
+  simp only [LLVM.Int.getValue_eq_getValueD]
+  simp
+  intro h2
+  simp [LLVM.Int.getValueD]
+  split
+  · simp [LLVM.Int.isPoison] at h2
+  · ext k hk
+    simp [BitVec.getLsbD_signExtend, BitVec.getElem_signExtend]
+    split
+    · simp [show k < 64 by omega, show k ≤ 15 by omega, ← BitVec.getLsbD_eq_getElem]
+    · simp [show k < 64 by omega]
+      bv_decide
+
+/--
+  Prove the correctness of the `sext` lowering pattern, with input width `i32`.
+-/
+theorem sext_refinement_32 {lhs : LLVM.Int 32} (h : 32 < w₂) (h' : w₂ ≤ 64) :
+    (Data.LLVM.Int.sext lhs w₂ h) ⊒ (RISCV.Reg.toInt (Data.RISCV.sextw (LLVM.Int.toReg lhs)) w₂) := by
+  simp only [llvm_toBitVec, reg_toBitVec]
+  simp only [LLVM.Int.getValue_eq_getValueD]
+  simp
+  intro h2
+  simp [LLVM.Int.getValueD]
+  split
+  · simp [LLVM.Int.isPoison] at h2
+  · ext k hk
+    simp [BitVec.getLsbD_signExtend, BitVec.getElem_signExtend]
+    split
+    · simp [show k < 64 by omega,  ← BitVec.getLsbD_eq_getElem]
+    · simp [show k < 64 by omega]
+
+/--
+  Prove the correctness of the `sext` lowering pattern, with input width different than `i8/i16/i32`.
+-/
+theorem sext_refinement {lhs : LLVM.Int w₁} (h : w₁ < w₂) (h' : w₂ ≤ 64) (h'' : w₁ ≠ 8 ∧ w₁ ≠ 16 ∧ w₁ ≠ 32) :
+    (Data.LLVM.Int.sext lhs w₂ h) ⊒
+      (RISCV.Reg.toInt (Data.RISCV.srai (64 - w₁) (Data.RISCV.slli (64 - w₁) (LLVM.Int.toReg lhs))) w₂) := by
+  simp only [llvm_toBitVec, reg_toBitVec]
+  simp only [LLVM.Int.getValue_eq_getValueD]
+  simp
+  by_cases hw₁ : w₁ = 0
+  · subst hw₁
+    simp
+    sorry
+  intro h2
+  simp [LLVM.Int.getValueD]
+  split
+  · simp [LLVM.Int.isPoison] at h2
+  · ext k hk
+    simp [← BitVec.getLsbD_eq_getElem, hk]
+    rw [Nat.mod_eq_of_lt (by rw [Nat.mod_eq_of_lt (by grind)]; grind)]
+    rw [Nat.mod_eq_of_lt (by grind)]
+
+    sorry
